RHL_Untyped.thy
@@ -9,7 +9,7 @@ definition rhoare_untyped :: "(memory \<Rightarrow> memory \<Rightarrow> bool) \
         \<and> apply_to_distr snd \<mu> = denotation_untyped c2 m2
         \<and> (\<forall>m1' m2'. (m1',m2') \<in> support_distr \<mu> \<longrightarrow> post m1' m2')))"
 
-definition rhoare_denotation :: "(memory \<Rightarrow> memory \<Rightarrow> bool) \<Rightarrow> _ \<Rightarrow> _ \<Rightarrow> (memory \<Rightarrow> memory \<Rightarrow> bool) \<Rightarrow> bool" where
+definition rhoare_denotation :: "('a \<Rightarrow> 'b \<Rightarrow> bool) \<Rightarrow> _ \<Rightarrow> _ \<Rightarrow> ('a \<Rightarrow> 'b \<Rightarrow> bool) \<Rightarrow> bool" where
   "rhoare_denotation pre c1 c2 post =
   (\<forall>m1 m2. pre m1 m2 \<longrightarrow> 
      (\<exists>\<mu>. apply_to_distr fst \<mu> = c1 m1
@@ -403,13 +403,19 @@ proof -
 qed
 *)
 
-lemma foldr_commute: 
+lemma foldr_commute:  (* TODO used? *)
   assumes "\<And>x y. f (g x y) = g' x (f y)"
   shows "f (foldr g l a) = foldr g' l (f a)"
     apply (induction l)
     using assms by auto
 
-lemma foldr_o: 
+lemma foldl_commute: 
+  assumes "\<And>x y. f (g x y) = g' (f x) y"
+  shows "f (foldl g a l) = foldl g' (f a) l"
+    apply (induction l rule:rev_induct)
+    using assms by auto
+
+lemma foldr_o:  (* TODO used? *)
   shows "(foldr (\<lambda>x. op o (f x)) l a) m = foldr f l (a m)"
   by (induction l, auto)
 
@@ -423,6 +429,478 @@ apply (metis list.exhaust list.sel(1) list.sel(3) prod.sel(1) zip_Cons_Cons zip_
 apply (induction bs arbitrary: as, auto)
 by (metis Pair_inject list.distinct(2) list.exhaust list.inject zip_Cons_Cons zip_Nil)
 
+definition "assign_default = foldl (\<lambda>p v. Seq p (Assign (pattern_1var v) 
+                      (const_expression_untyped (vu_type v) (t_default (vu_type v))))) Skip"
+
+
+(* TODO move *)
+lemma memory_lookup_update_pattern_notsame:
+  assumes "x \<notin> set (pu_vars p)"
+  shows "memory_lookup_untyped (memory_update_untyped_pattern m p a) x = memory_lookup_untyped m x"
+proof -
+  def vg == "pu_var_getters p"
+  hence vg: "x \<notin> fst ` set vg"
+    using assms pu_var_getters_def pu_vars_def by auto
+  show ?thesis
+    unfolding memory_update_untyped_pattern_def  vg_def[symmetric]
+    apply (insert vg)
+    apply (induct vg rule:rev_induct)
+     by (auto simp: memory_lookup_update_notsame_untyped)
+qed
+
+
+lemma callproc_rule:
+  fixes body pargs ret x args
+    and V -- "variables that our observational equivalence talks about"
+    and locals -- "(superset of) local variables of the procedure"
+    and non_parg_locals -- "(superset of) locals without variables from pargs"
+  defines "p == Proc body pargs ret"
+  defines "G == {x\<in>V. vu_global x}"
+  
+  assumes body_locals: "\<And>x. \<lbrakk> x\<in>set(vars_untyped body); \<not> vu_global x \<rbrakk> \<Longrightarrow> x\<in>set locals"
+  assumes pargs_locals: "\<And>x. x\<in>set (pu_vars pargs) \<Longrightarrow> \<not> vu_global x \<Longrightarrow> x\<in>set locals"
+  assumes ret_locals: "\<And>x. \<lbrakk> x\<in>set(eu_vars ret); \<not> vu_global x \<rbrakk> \<Longrightarrow> x\<in>set locals"
+  assumes locals_local: "\<And>x. x\<in>set locals \<Longrightarrow> \<not> vu_global x"
+(*  assumes argvars_locals: "\<And>e x. e\<in>set (eu_vars args) \<Longrightarrow> x\<in>set(eu_vars e) \<Longrightarrow> x\<notin>set locals" *)
+  assumes localsV: "V \<inter> set locals \<subseteq> set (pu_vars x)"
+  assumes globalsVbody: "\<And>x. x\<in>set(vars_untyped body) \<Longrightarrow> vu_global x \<Longrightarrow> x\<in>V"
+  assumes globalsVret: "\<And>x. x\<in>set(eu_vars ret) \<Longrightarrow> vu_global x \<Longrightarrow> x\<in>V"
+  assumes argvarsV: "set(eu_vars args) \<subseteq> V"
+  assumes non_parg_locals: "set non_parg_locals = set locals - set (pu_vars pargs)"
+(*
+| denotation_untyped_CallProc: "denotation_untyped (CallProc v (Proc body pargs return) args) m = 
+  (let argval = eu_fun args m in
+  let m' = init_locals m in
+  let m' = memory_update_untyped_pattern m' pargs argval in
+  apply_to_distr (\<lambda>m'.
+    let res = eu_fun return m' in
+    let m' = restore_locals m m' in
+    memory_update_untyped_pattern m' v res)
+  (denotation_untyped body m'))"
+*)
+  defines "unfolded == Seq (Seq (Seq (Assign pargs args) (assign_default non_parg_locals)) body)
+                           (Assign x ret)"
+  shows "obs_eq_untyped V V (CallProc x p args) unfolded"
+proof (unfold obs_eq_untyped_def rhoare_untyped_rhoare_denotation, rule rhoare_denotation_post_eq)
+  fix m1 m2 assume eq_init: "\<forall>x\<in>V. memory_lookup_untyped m1 x = memory_lookup_untyped m2 x"
+
+  def eq == "\<lambda>V \<mu> \<nu>. apply_to_distr (\<lambda>m x. if x \<in> V then memory_lookup_untyped m x else undefined) \<mu>
+                   = apply_to_distr (\<lambda>m x. if x \<in> V then memory_lookup_untyped m x else undefined) \<nu>" (* TODO remove *)
+(*  have "eq = (\<lambda>V \<mu> \<nu>. apply_to_distr (\<lambda>m x. if x \<in> V then memory_lookup_untyped m x else undefined) \<mu>
+                   = apply_to_distr (\<lambda>m x. if x \<in> V then memory_lookup_untyped m x else undefined) \<nu>)" *)
+(*  def eq == "\<lambda>X c1 c2. rhoare_denotation (\<lambda>m1 m2. \<forall>x\<in>V. memory_lookup_untyped m1 x = memory_lookup_untyped m2 x)
+                                         c1 c2
+                                         (\<lambda>m1 m2. \<forall>x\<in>X. memory_lookup_untyped m1 x = memory_lookup_untyped m2 x)" 
+  have eq_mono: "\<And>A B c1 c2. A \<subseteq> B \<Longrightarrow> eq B c1 c2 \<Longrightarrow> eq A c1 c2" 
+    unfolding eq_def rhoare_denotation_def by blast *)
+
+  def argvars == "set (eu_vars args)"
+
+  def untouched == "\<lambda>V \<mu>. \<forall>m\<in>support_distr \<mu>. \<forall>x\<in>V. memory_lookup_untyped m x = memory_lookup_untyped m2 x"
+(*  def G == "{x\<in>V. vu_global x} :: variable_untyped set" *)
+  def co_locals == "{x. \<not>vu_global x \<and> x\<notin>set locals}"
+
+  def cp1 == "point_distr (memory_update_untyped_pattern (init_locals m1) pargs (eu_fun args m1))"
+  def uf1 == "denotation_untyped (Seq (Assign pargs args) (assign_default non_parg_locals)) m2"
+
+(*  def uf1_1 == "foldl (\<lambda>m (v, f). memory_update_untyped m v (f (eu_fun args m2))) m2 (pu_var_getters pargs)" *)
+  def uf1_1 == "memory_update_untyped_pattern m2 pargs (eu_fun args m2)"
+  def uf1_2 == "\<lambda>m2. foldl (\<lambda>m v. (\<lambda>m x. memory_update_untyped m x
+               (eu_fun (const_expression_untyped (vu_type x) (t_default (vu_type x))) m)) m v) m2 non_parg_locals"
+  have uf1: "uf1 = point_distr (uf1_2 uf1_1)"
+  proof -
+    have "denotation_untyped (Assign pargs args) m2 = point_distr uf1_1"
+      by (simp add: memory_update_untyped_pattern_def uf1_1_def)
+    hence l1: "uf1 = denotation_untyped (assign_default non_parg_locals) uf1_1"
+      using uf1_def by fastforce
+    have "denotation_untyped (assign_default non_parg_locals) uf1_1 = point_distr (uf1_2 uf1_1)"
+      unfolding assign_default_def uf1_2_def
+      apply (induct non_parg_locals rule: rev_induct) by auto
+    with l1 show "uf1 = point_distr (uf1_2 uf1_1)" by simp
+  qed
+
+  have eq1: "eq (G\<union>set locals) cp1 uf1"
+  proof (unfold eq_def)
+(*  proof (unfold eq_def, rule rhoare_denotation_post_eq) *)
+(*    assume init_eqV: "\<forall>x\<in>V. memory_lookup_untyped m1 x = memory_lookup_untyped m2 x" *)
+    def cp1mem == "memory_update_untyped_pattern (init_locals m1) pargs (eu_fun args m1)"
+    have cp1mem_uf: "\<forall>x\<in>(G\<union>set locals). memory_lookup_untyped cp1mem x = memory_lookup_untyped (uf1_2 (uf1_1)) x"
+    proof
+      fix x assume "x \<in> G \<union> set locals" 
+      hence cases: "\<And>P. \<lbrakk> \<lbrakk> x \<notin> set (pu_vars pargs); x\<in>G \<rbrakk> \<Longrightarrow> P; 
+                          \<lbrakk> x \<notin> set (pu_vars pargs); x\<in>set locals \<rbrakk> \<Longrightarrow> P; 
+                          x \<in> set (pu_vars pargs) \<Longrightarrow> P \<rbrakk> \<Longrightarrow> P"  by auto
+      show "memory_lookup_untyped cp1mem x = memory_lookup_untyped (uf1_2 (uf1_1)) x"
+      proof (rule cases)
+        assume "x \<in> G" and not_pargs: "x \<notin> set (pu_vars pargs)"
+        hence "x \<in> V" using G_def by auto
+        from `x \<in> G` have "vu_global x" by (simp add: G_def)
+        have init: "memory_lookup_untyped (init_locals m1) x = memory_lookup_untyped m1 x"
+          unfolding init_locals_def memory_lookup_untyped_def apply (simp add: `vu_global x`)
+          apply (subst Abs_memory_inverse) using Rep_memory by auto
+        have cp: "memory_lookup_untyped cp1mem x = memory_lookup_untyped m1 x" 
+          unfolding cp1mem_def apply (subst memory_lookup_update_pattern_notsame)
+          using not_pargs init .
+        have uf_vg: "memory_lookup_untyped uf1_1 x == memory_lookup_untyped m2 x"
+          unfolding uf1_1_def apply (subst memory_lookup_update_pattern_notsame)
+          using not_pargs by blast
+        have "x \<notin> set non_parg_locals"
+          using `vu_global x` locals_local non_parg_locals by auto
+        have uf: "memory_lookup_untyped (uf1_2 (uf1_1)) x = memory_lookup_untyped m2 x"
+          unfolding uf1_2_def apply (insert `x \<notin> set non_parg_locals`)
+          apply (induct non_parg_locals rule:rev_induct)
+            close (auto simp: uf_vg)
+          by (auto simp: memory_lookup_update_notsame_untyped)
+        from cp uf eq_init `x\<in>V` show ?thesis by auto
+      next
+        assume "x \<in> set locals" and x_nin_pargs: "x \<notin> set (pu_vars pargs)"
+        hence x_parg_non_locals: "x \<in> set non_parg_locals"
+          by (simp add: non_parg_locals)
+        have "\<not> vu_global x"
+          by (simp add: `x \<in> set locals` locals_local)
+        have init: "memory_lookup_untyped (init_locals m1) x = t_default (vu_type x)"
+          unfolding init_locals_def memory_lookup_untyped_def using `\<not> vu_global x` apply auto
+          apply (subst Abs_memory_inverse) using Rep_memory by auto
+        have cp: "memory_lookup_untyped cp1mem x = t_default (vu_type x)"
+          unfolding cp1mem_def 
+          apply (subst memory_lookup_update_pattern_notsame) using x_nin_pargs init .
+        have uf: "memory_lookup_untyped (uf1_2 uf1_1) x = t_default (vu_type x)"
+          unfolding uf1_2_def apply (insert x_parg_non_locals, induct non_parg_locals rule:rev_induct)
+          by (auto simp: eu_fun_const_expression_untyped memory_lookup_update_untyped)
+        from cp uf show ?thesis by auto
+      next
+        assume xpargs: "x \<in> set (pu_vars pargs)"
+        def vg == "pu_var_getters pargs"
+        have vg: "\<exists>(v,g)\<in>set vg. v=x"
+          using xpargs unfolding vg_def pu_vars_def by fastforce
+        have "memory_lookup_untyped cp1mem x = memory_lookup_untyped (uf1_1) x"
+          unfolding cp1mem_def memory_update_untyped_pattern_def uf1_1_def vg_def[symmetric]
+          proof (insert vg, induction vg rule:rev_induct) 
+          case Nil thus ?case by auto
+          next case snoc show ?case apply auto
+            by (smt Un_iff argvarsV case_prod_unfold empty_iff eq_init eu_fun_footprint insert_iff list.set(1) list.set(2) memory_lookup_update_untyped set_append snoc.IH snoc.prems subsetCE)
+          qed
+        moreover
+        have x_nin_parg_locals: "x \<notin> set non_parg_locals"
+          by (simp add: xpargs non_parg_locals)
+        have "memory_lookup_untyped (uf1_1) x = memory_lookup_untyped (uf1_2 uf1_1) x"
+          unfolding uf1_2_def apply (insert x_nin_parg_locals, induct non_parg_locals rule:rev_induct)
+          using memory_lookup_update_untyped by auto
+        finally show ?thesis.
+      qed
+    qed
+
+    show "apply_to_distr (\<lambda>m x. if x \<in> G \<union> set locals then memory_lookup_untyped m x else undefined) (cp1) =
+          apply_to_distr (\<lambda>m x. if x \<in> G \<union> set locals then memory_lookup_untyped m x else undefined) (uf1)"
+      unfolding cp1_def cp1mem_def[symmetric] uf1 apply simp
+      apply (rule cong[OF refl[of point_distr]])
+      using cp1mem_uf by force
+  qed
+
+  have untouched1: "untouched co_locals uf1"
+  proof (unfold uf1 untouched_def co_locals_def, auto)
+    fix x assume "\<not> vu_global x" and "x \<notin> set locals"
+    hence x_nin_pargs: "x \<notin> set (pu_vars pargs)" using pargs_locals by blast 
+    have uf_vg: "memory_lookup_untyped uf1_1 x == memory_lookup_untyped m2 x"
+      unfolding uf1_1_def apply (subst memory_lookup_update_pattern_notsame)
+      by (simp_all add: x_nin_pargs)
+    have "x \<notin> set non_parg_locals"
+      using `x \<notin> set locals` non_parg_locals by auto
+    show "memory_lookup_untyped (uf1_2 (uf1_1)) x = memory_lookup_untyped m2 x"
+      unfolding uf1_2_def apply (insert `x \<notin> set non_parg_locals`)
+      apply (induct non_parg_locals rule:rev_induct)
+        close (auto simp: uf_vg)
+      by (auto simp: memory_lookup_update_notsame_untyped)
+  qed
+
+  def uf2 == "compose_distr (denotation_untyped body) uf1"
+  def cp2 == "compose_distr (denotation_untyped body) cp1"
+
+  have eq_body: "obs_eq_untyped (G\<union>set locals) (G\<union>set locals) body body"
+    apply (rule self_obseq_vars, rule, case_tac "x\<in>G", simp)
+    apply auto using globalsVbody body_locals unfolding  G_def by auto
+
+  have eq_compose': "\<And>P X Y \<mu> \<nu> f g. 
+     eq X \<mu> \<nu> \<Longrightarrow> (\<forall>m\<in>support_distr \<nu>. P m) \<Longrightarrow> (\<exists>m. P m)
+     \<Longrightarrow> rhoare_denotation (\<lambda>m1 m2. (\<forall>x\<in>X. memory_lookup_untyped m1 x = memory_lookup_untyped m2 x) 
+        \<and> P m2) f g
+     (\<lambda>m1 m2. \<forall>x\<in>Y. memory_lookup_untyped m1 x = memory_lookup_untyped m2 x) \<Longrightarrow>
+     eq Y (compose_distr f \<mu>) (compose_distr g \<nu>)"
+  proof -
+    fix X Y \<mu> \<nu> f g P
+    assume eq: "eq X \<mu> \<nu>"
+    assume P: "\<forall>m\<in>support_distr \<nu>. P m"
+    assume "\<exists>m. P m" then obtain m0 where "P m0" by auto
+    assume eq2: "rhoare_denotation (\<lambda>m1 m2. (\<forall>x\<in>X. memory_lookup_untyped m1 x = memory_lookup_untyped m2 x) \<and> P m2) f g
+     (\<lambda>m1 m2. \<forall>x\<in>Y. memory_lookup_untyped m1 x = memory_lookup_untyped m2 x)"
+    have rd1: "rhoare_denotation (\<lambda>m1' m2'. m1'=m0 \<and> m2'=m0)
+          (\<lambda>m. if m=m0 then \<mu> else 0) (\<lambda>m. if m=m0 then \<nu> else 0)
+          (\<lambda>m1 m2. \<forall>x\<in>X. memory_lookup_untyped m1 x = memory_lookup_untyped m2 x)"
+      apply (rule rhoare_denotation_post_eq) using eq unfolding eq_def by auto
+(*    have rd2: "rhoare_denotation (\<lambda>m1' m2'. m1'=m0 \<and> m2'=m0)
+          (\<lambda>m. if m=m0 then \<mu> else 0) (\<lambda>m. if m=m0 then \<nu> else 0)
+          (\<lambda>m1 m2. P m2)"
+      unfolding rhoare_denotation_def apply auto
+      apply (rule exI[of _ "product_distr \<mu> \<nu>"])
+      apply auto
+      by later *)
+    have "rhoare_denotation (\<lambda>m1' m2'. m1'=m0 \<and> m2'=m0)
+          (\<lambda>m. if m=m0 then \<mu> else 0) (\<lambda>m. if m=m0 then \<nu> else 0)
+          (\<lambda>m1 m2. (\<forall>x\<in>X. memory_lookup_untyped m1 x = memory_lookup_untyped m2 x) \<and> P m2)"
+    proof -
+      obtain \<mu>' where \<mu>: "apply_to_distr fst \<mu>' = \<mu>" and \<nu>: "apply_to_distr snd \<mu>' = \<nu>" 
+        and post: "\<And>m1' m2'. (m1', m2') \<in> support_distr \<mu>' \<Longrightarrow> (\<forall>x\<in>X. memory_lookup_untyped m1' x = memory_lookup_untyped m2' x)"
+        using rd1 unfolding rhoare_denotation_def by auto
+      have P': "\<And>m1' m2'. (m1', m2') \<in> support_distr \<mu>' \<Longrightarrow> P m2'"
+        using P \<nu> by fastforce
+      show ?thesis
+        unfolding rhoare_denotation_def apply simp apply (rule exI[of _ \<mu>'])
+        using \<mu> \<nu> post P' by auto
+    qed
+    hence rhd: "rhoare_denotation (\<lambda>m1' m2'. m1'=m0 \<and> m2'=m0)
+          (\<lambda>m. (compose_distr f ((\<lambda>m. if m=m0 then \<mu> else 0) m)))
+          (\<lambda>m. (compose_distr g ((\<lambda>m. if m=m0 then \<nu> else 0) m)))
+          (\<lambda>m1 m2. \<forall>x\<in>Y. memory_lookup_untyped m1 x = memory_lookup_untyped m2 x)"
+      apply (rule rseq_rule_denotation)
+      using eq2 unfolding obs_eq_untyped_def rhoare_untyped_rhoare_denotation.
+    show "eq Y (compose_distr f \<mu>) (compose_distr g \<nu>)"
+      unfolding eq_def cp2_def uf2_def
+      using rhoare_denotation_post_eq2[OF rhd] by simp
+  qed
+
+  have eq_compose: "\<And>X Y \<mu> \<nu> f g. 
+     eq X \<mu> \<nu> \<Longrightarrow> rhoare_denotation (\<lambda>m1 m2. \<forall>x\<in>X. memory_lookup_untyped m1 x = memory_lookup_untyped m2 x) f g
+     (\<lambda>m1 m2. \<forall>x\<in>Y. memory_lookup_untyped m1 x = memory_lookup_untyped m2 x) \<Longrightarrow>
+     eq Y (compose_distr f \<mu>) (compose_distr g \<nu>)"
+     by (rule_tac eq_compose', auto)
+(*  proof -
+    fix X Y \<mu> \<nu> f g
+    assume eq: "eq X \<mu> \<nu>"
+    assume eq2: "rhoare_denotation (\<lambda>m1 m2. \<forall>x\<in>X. memory_lookup_untyped m1 x = memory_lookup_untyped m2 x) f g
+     (\<lambda>m1 m2. \<forall>x\<in>Y. memory_lookup_untyped m1 x = memory_lookup_untyped m2 x)"
+    have "rhoare_denotation (\<lambda>m1' m2'. m1'=m1 \<and> m2'=m2)
+          (\<lambda>m. if m=m1 then \<mu> else 0) (\<lambda>m. if m=m2 then \<nu> else 0)
+          (\<lambda>m1 m2. \<forall>x\<in>X. memory_lookup_untyped m1 x = memory_lookup_untyped m2 x)"
+      apply (rule rhoare_denotation_post_eq) using eq unfolding eq_def by auto
+    hence rhd: "rhoare_denotation (\<lambda>m1' m2'. m1'=m1 \<and> m2'=m2)
+          (\<lambda>m. (compose_distr f ((\<lambda>m. if m=m1 then \<mu> else 0) m)))
+          (\<lambda>m. (compose_distr g ((\<lambda>m. if m=m2 then \<nu> else 0) m)))
+          (\<lambda>m1 m2. \<forall>x\<in>Y. memory_lookup_untyped m1 x = memory_lookup_untyped m2 x)"
+      apply (rule rseq_rule_denotation)
+      using eq2 unfolding obs_eq_untyped_def rhoare_untyped_rhoare_denotation.
+    show "eq Y (compose_distr f \<mu>) (compose_distr g \<nu>)"
+      unfolding eq_def cp2_def uf2_def
+      using rhoare_denotation_post_eq2[OF rhd] by simp
+  qed *)
+
+  have eq2: "eq (G\<union>set locals) cp2 uf2"
+    unfolding cp2_def uf2_def apply (rule eq_compose)
+    close (fact eq1) using eq_body unfolding obs_eq_untyped_def rhoare_untyped_rhoare_denotation .
+
+  have untouched2: "untouched co_locals uf2"
+  proof (unfold untouched_def uf2_def, auto)
+    fix m' m x
+    assume "m' \<in> support_distr (uf1)" and x_co: "x \<in> co_locals"
+    hence m'_m2: "memory_lookup_untyped m' x = memory_lookup_untyped m2 x"
+      using untouched1 unfolding untouched_def by auto
+    assume m: "m \<in> support_distr (denotation_untyped body m')"
+    have x: "x \<notin> set(vars_untyped body)"
+      using x_co body_locals unfolding co_locals_def by auto
+    have m_m': "memory_lookup_untyped m x = memory_lookup_untyped m' x"
+      apply (rule readonly_notin_vars[unfolded hoare_untyped_def, rule_format, where c=body and m=m'])
+      using m x by auto
+    with m'_m2 show "memory_lookup_untyped m x = memory_lookup_untyped m2 x" by simp
+  qed
+
+  def uf3mem == "\<lambda>m. memory_update_untyped_pattern m x (eu_fun ret m)"
+  def uf3 == "compose_distr (denotation_untyped (Assign x ret)) uf2"
+  def cp3mem == "\<lambda>m'. let res = eu_fun ret m' in let m' = restore_locals m1 m' in
+    memory_update_untyped_pattern m' x res"
+  def cp3 == "apply_to_distr cp3mem cp2"
+  
+  have cp3: "cp3 = denotation_untyped (CallProc x p args) m1" 
+    unfolding cp3_def cp3mem_def cp2_def p_def cp1_def by simp
+  have uf3: "uf3 = denotation_untyped unfolded m2"
+    unfolding uf3_def unfolded_def p_def uf2_def uf1_def by simp
+
+  have uf3': "uf3 = apply_to_distr uf3mem uf2"
+    unfolding uf3_def uf3mem_def denotation_untyped_Assign[THEN ext[of "denotation_untyped (Assign _ _)"]]
+    by simp
+
+  have eq3_almost: "\<And>m1' m2' y. 
+            \<forall>x\<in>G \<union> set locals. memory_lookup_untyped m1' x = memory_lookup_untyped m2' x
+        \<Longrightarrow> \<forall>x\<in>co_locals. memory_lookup_untyped m2' x = memory_lookup_untyped m2 x
+        \<Longrightarrow> y \<in> V
+        \<Longrightarrow> memory_lookup_untyped (cp3mem m1') y = memory_lookup_untyped (uf3mem m2') y"
+  proof -
+    fix m1' m2' y assume m'_eq: "\<forall>x\<in>G \<union> set locals. memory_lookup_untyped m1' x = memory_lookup_untyped m2' x"
+    assume untouched: "\<forall>x\<in>co_locals. memory_lookup_untyped m2' x = memory_lookup_untyped m2 x"
+    assume yV: "y \<in> V" (* ? cases:
+      y \<in> set (pu_vars x) <- the return pattern:  then both sides get updated the same
+      y \<in> non_parg_locals: should not happen (by y\<in>V) ?
+      y \<in> co_locals: using "untouched2"
+      y : globals - pu_vars x
+    *)
+    hence cases: "\<And>P. \<lbrakk> y \<in> set (pu_vars x) \<Longrightarrow> P; 
+                        \<lbrakk> y \<in> co_locals; y\<notin>set(pu_vars x) \<rbrakk> \<Longrightarrow> P; 
+                        \<lbrakk> vu_global y; y \<notin> set (pu_vars x) \<rbrakk> \<Longrightarrow> P \<rbrakk> \<Longrightarrow> P"
+      apply atomize_elim unfolding co_locals_def G_def using localsV by auto
+    show "memory_lookup_untyped (cp3mem m1') y = memory_lookup_untyped (uf3mem m2') y"
+    proof (rule cases)
+      assume y_pu_vars: "y \<in> set (pu_vars x)" 
+      def vg == "pu_var_getters x"
+      have vg: "\<exists>(v,g)\<in>set vg. v=y"
+        using y_pu_vars unfolding vg_def pu_vars_def by fastforce
+      show "memory_lookup_untyped (cp3mem m1') y = memory_lookup_untyped (uf3mem m2') y"
+        unfolding cp3mem_def memory_update_untyped_pattern_def uf3mem_def vg_def[symmetric] apply simp
+      proof (insert vg, induction vg rule:rev_induct) 
+        case Nil thus ?case by auto
+        next case snoc show ?case apply auto
+          by (smt G_def Un_iff `\<forall>x\<in>G \<union> set locals. memory_lookup_untyped m1' x = memory_lookup_untyped m2' x` case_prod_unfold empty_iff eu_fun_footprint globalsVret insert_iff list.set(1) list.set(2) mem_Collect_eq memory_lookup_update_untyped ret_locals set_append snoc.IH snoc.prems)
+      qed
+    next
+      assume y_co_locals: "y \<in> co_locals" and y_nin_pu_vars: "y\<notin>set(pu_vars x)"
+      hence y_local: "\<not> vu_global y" by (simp add: co_locals_def)
+      have restore_locals: "memory_lookup_untyped (restore_locals m1 m1') y = memory_lookup_untyped m1 y"
+        unfolding restore_locals_def memory_lookup_untyped_def apply (simp add: y_local)
+        apply (subst Abs_memory_inverse) using Rep_memory by auto
+      have "memory_lookup_untyped (uf3mem m2') y = memory_lookup_untyped m2' y" 
+        unfolding uf3mem_def apply (subst memory_lookup_update_pattern_notsame) using y_co_locals y_nin_pu_vars by auto
+      also have "\<dots> = memory_lookup_untyped m2 y"
+        using `y \<in> co_locals` untouched by auto
+      also have "\<dots> = memory_lookup_untyped m1 y"
+        using `y \<in> V` eq_init by auto
+      also have "memory_lookup_untyped (cp3mem m1') y = memory_lookup_untyped m1 y"
+        unfolding cp3mem_def apply (simp, subst memory_lookup_update_pattern_notsame) 
+        using restore_locals y_nin_pu_vars by auto
+      ultimately show ?thesis by simp
+    next
+      assume y_global: "vu_global y" and y_nin_pu_vars: "y \<notin> set (pu_vars x)"
+      have restore_locals: "memory_lookup_untyped (restore_locals m1 m1') y = memory_lookup_untyped m1' y"
+        unfolding restore_locals_def memory_lookup_untyped_def apply (simp add: y_global)
+        apply (subst Abs_memory_inverse) using Rep_memory by auto
+      have "memory_lookup_untyped (uf3mem m2') y = memory_lookup_untyped m2' y" 
+        unfolding uf3mem_def apply (subst memory_lookup_update_pattern_notsame) using y_nin_pu_vars by auto
+      also have "\<dots> = memory_lookup_untyped m1' y"
+        using G_def m'_eq yV y_global by force
+      also have "\<dots> = memory_lookup_untyped (cp3mem m1') y"
+        unfolding cp3mem_def apply simp apply (subst memory_lookup_update_pattern_notsame)
+        using y_nin_pu_vars restore_locals by simp_all
+      finally show ?thesis ..
+    qed
+  qed
+
+  have eq3_almost': "\<And>m1' m2' y. (\<forall>x\<in>G \<union> set locals. memory_lookup_untyped m1' x = memory_lookup_untyped m2' x)
+        \<and> (\<forall>x\<in>co_locals. memory_lookup_untyped m2' x = memory_lookup_untyped m2 x)
+    \<Longrightarrow> 
+              (\<lambda>x. if x \<in> V then memory_lookup_untyped (cp3mem m1') x else undefined) =
+              (\<lambda>x. if x \<in> V then memory_lookup_untyped (uf3mem m2') x else undefined)"
+    using eq3_almost by auto
+
+  have eq3: "eq V cp3 uf3"
+    unfolding uf3' cp3_def  compose_point_distr_l[symmetric]
+    apply (rule eq_compose'[where P="\<lambda>m. \<forall>x\<in>co_locals. memory_lookup_untyped m x = memory_lookup_untyped m2 x"])
+       close (fact eq2)
+      using untouched2 close (auto simp: untouched_def)
+     close (rule exI[of _ m2], simp)
+    apply (rule rhoare_denotation_post_eq, simp)
+    apply (subst eq3_almost') by auto
+
+  from eq3 cp3 uf3
+  show "apply_to_distr (\<lambda>m x. if x \<in> V then memory_lookup_untyped m x else undefined) (denotation_untyped (CallProc x p args) m1) =
+        apply_to_distr (\<lambda>m x. if x \<in> V then memory_lookup_untyped m x else undefined) (denotation_untyped unfolded m2)" 
+    unfolding eq_def by simp
+qed
+
+(*
+  have 
+
+  have eq_assign: "obs_eq_untyped (G\<union>set locals) (G\<union>set locals\<union>{x}) (Assign (pattern_1var x) ret) (Assign (pattern_1var x) ret)"
+    apply (rule self_obseq_assign)
+    using globalsVret ret_locals unfolding G_def by auto
+  have eq3: "eq (G\<union>set locals\<union>{x}) cp3 uf3"
+    unfolding eq_def uf3_def cp3_def
+    apply (rule rseq_rule_denotation)
+      close (fact eq2[unfolded eq_def])
+      using eq_assign unfolding obs_eq_untyped_def rhoare_untyped_rhoare_denotation .
+  have untouched3: "untouched (co_locals-{x}) uf3"
+  proof (unfold untouched_def uf3_def, rule+, auto)
+    fix m0 m y
+    assume "m \<in> support_distr (uf2 m0)" and y_co: "y \<in> co_locals"
+    hence m'_m0: "memory_lookup_untyped m y = memory_lookup_untyped m0 y"
+      using untouched2 unfolding untouched_def by auto
+    assume yx: "y\<noteq>x"
+    have m_m': "memory_lookup_untyped (memory_update_untyped m x (eu_fun ret m)) y = memory_lookup_untyped m y"
+      apply (rule readonly_assign[unfolded hoare_untyped_def, rule_format, where x="pattern_1var x" and e=ret and y=y and m=m])
+      using yx by auto 
+    with m'_m0 show "memory_lookup_untyped (memory_update_untyped m x (eu_fun ret m)) y = memory_lookup_untyped m0 y" by simp
+  qed
+  
+  def cp4 == "\<lambda>m. apply_to_distr (restore_locals x m) (cp3 m)"
+
+  have eq_uf3_cp4: "eq V cp4 uf3"
+  proof (unfold eq_def, rule rhoare_denotation_post_eq)
+    fix m1 m2 assume m1m2: "\<forall>x\<in>V. memory_lookup_untyped m1 x = memory_lookup_untyped m2 x"
+    hence m1m2': "\<And>x. x\<in>V \<Longrightarrow> memory_lookup_untyped m1 x = memory_lookup_untyped m2 x" by auto
+    def m1' == "memory_lookup_untyped m1"
+    def restore == "\<lambda>newmem (y::variable_untyped). 
+      if x=y then newmem y else
+      if vu_global y then newmem y else
+      m1' y :: val"
+      
+    def proj1 == "\<lambda>m y. if y \<in> G\<union>set locals\<union>{x} then m y else (undefined::val)"
+    def proj2 == "\<lambda>m y. if y \<in> V then m y else (undefined::val)"
+    have memfuns: "(\<lambda>m y. if y \<in> V then memory_lookup_untyped m y else undefined) o (restore_locals x m1)
+                   = proj2 o restore o memory_lookup_untyped"
+      unfolding proj2_def restore_def o_def restore_locals_lookup m1'_def by force
+    have add_proj1: "proj2 o restore = proj2 o restore o proj1"
+      unfolding proj2_def proj1_def restore_def o_def 
+      apply (rule ext, rule ext) using G_def by auto
+    have eq_cp_uf: "apply_to_distr (proj1 o memory_lookup_untyped) (cp3 m1) = apply_to_distr (proj1 o memory_lookup_untyped) (uf3 m2)"
+      using eq3 m1m2 unfolding proj1_def eq_def o_def by (rule rhoare_denotation_post_eq2)
+    have rm_restore: "\<And>m. (\<forall>y\<in>(co_locals-{x})\<inter>V. m y = m1' y) \<Longrightarrow> (proj2 o restore o proj1) m = proj2 m"
+      unfolding proj2_def restore_def proj1_def apply (rule ext) apply auto
+      using G_def close blast
+      using localsV close auto
+      using G_def close blast
+      by (metis (full_types, lifting) IntI co_locals_def' mem_Collect_eq member_remove remove_def)
+    have supp: "\<And>m. m \<in> support_distr (uf3 m2) \<Longrightarrow> \<forall>x\<in>(co_locals-{x})\<inter>V. memory_lookup_untyped m x = memory_lookup_untyped m1 x"
+      apply (rule ballI)
+      apply (subst m1m2') close auto
+      using untouched3 untouched_def by blast
+
+    show "apply_to_distr (\<lambda>m y. if y\<in>V then memory_lookup_untyped m y else undefined) (cp4 m1)
+        = apply_to_distr (\<lambda>m y. if y\<in>V then memory_lookup_untyped m y else undefined) (uf3 m2)"
+      unfolding cp4_def
+      apply (subst apply_to_distr_twice)
+      apply (subst memfuns[unfolded o_def])
+      apply (subst add_proj1[unfolded o_def, THEN cong, OF refl])
+      apply (subst apply_to_distr_twice[symmetric, where f="\<lambda>m. proj2(restore m)"])
+      apply (subst eq_cp_uf[unfolded o_def])
+      apply (subst apply_to_distr_twice)
+      apply (subst apply_to_distr_cong)
+       apply (rule rm_restore[unfolded o_def]) using supp close (simp add: m1'_def)
+      unfolding proj2_def by simp
+  qed
+
+
+
+  have uf3_unfolded: "uf3 = denotation_untyped unfolded"
+    unfolding uf3_def unfolded_def uf2_def uf1_def by auto
+  have cp4_callproc: "cp4 = denotation_untyped (CallProc x p args)"
+    unfolding cp1_def cp2_def cp3_def cp4_def p_def
+    unfolding denotation_untyped_CallProc[THEN ext]
+              denotation_untyped_Assign[THEN ext]
+    by auto
+
+  show "obs_eq_untyped V V (CallProc x p args) unfolded"
+    unfolding obs_eq_untyped_def rhoare_untyped_rhoare_denotation
+    unfolding uf3_unfolded[symmetric] cp4_callproc[symmetric]
+    using eq_uf3_cp4 unfolding eq_def by simp
+qed 
+*)
+
+(*
 lemma callproc_rule:
   fixes body pargs ret x args V locals
   defines "p == Proc body pargs ret"
@@ -758,6 +1236,8 @@ proof -
     unfolding uf3_unfolded[symmetric] cp4_callproc[symmetric]
     using eq_uf3_cp4 unfolding eq_def by simp
 qed 
+*)
+
 
 (*
 lemma rseq_rule1:
